Cpc/Spec.lean
@@ -253,7 +253,7 @@ def __eo_to_smt : Term -> SmtTerm
   | (Term.Apply (Term.UOp UserOp._at_mod_by_zero) x1) => (SmtTerm.mod (__eo_to_smt x1) (SmtTerm.Numeral 0))
   | (Term.Apply (Term.Apply (Term.UOp UserOp.select) x1) x2) => (SmtTerm.select (__eo_to_smt x1) (__eo_to_smt x2))
   | (Term.Apply (Term.Apply (Term.Apply (Term.UOp UserOp.store) x1) x2) x3) => (SmtTerm.store (__eo_to_smt x1) (__eo_to_smt x2) (__eo_to_smt x3))
-  | (Term.UOp2 UserOp2._at_array_deq_diff x1 x2) => 
+  | (Term.Apply (Term.Apply (Term.UOp UserOp._at_array_deq_diff) x1) x2) => 
     let _v0 := (__eo_to_smt x2)
     let _v1 := (__eo_to_smt x1)
     (__eo_to_smt_array_deq_diff _v1 (__smtx_typeof _v1) _v0 (__smtx_typeof _v0))
@@ -361,13 +361,13 @@ def __eo_to_smt : Term -> SmtTerm
   | (Term.Apply (Term.UOp UserOp.seq_unit) x1) => (SmtTerm.seq_unit (__eo_to_smt x1))
   | (Term.Apply (Term.Apply (Term.UOp UserOp.seq_nth) x1) x2) => (SmtTerm.seq_nth (__eo_to_smt x1) (__eo_to_smt x2))
   | (Term.UOp3 UserOp3._at_re_unfold_pos_component x1 x2 x3) => (native_ite (__eo_to_smt_nat_is_valid x3) (__eo_to_smt_re_unfold_pos_component (__eo_to_smt x1) (__eo_to_smt x2) (__eo_to_smt_nat x3)) SmtTerm.None)
-  | (Term.UOp2 UserOp2._at_strings_deq_diff x1 x2) => 
+  | (Term.Apply (Term.Apply (Term.UOp UserOp._at_strings_deq_diff) x1) x2) => 
     let _v0 := (SmtTerm.Numeral 1)
     let _v2 := (SmtTerm.Var (native_string_lit "@x") SmtType.Int)
     (SmtTerm.choice_nth (native_string_lit "@x") SmtType.Int (SmtTerm.not (SmtTerm.eq (SmtTerm.str_substr (__eo_to_smt x1) _v2 _v0) (SmtTerm.str_substr (__eo_to_smt x2) _v2 _v0))) native_nat_zero)
-  | (Term.Apply (Term.UOp1 UserOp1._at_strings_stoi_result x1) x2) => (SmtTerm.str_to_int (SmtTerm.str_substr (__eo_to_smt x1) (SmtTerm.Numeral 0) (__eo_to_smt x2)))
-  | (Term.UOp1 UserOp1._at_strings_stoi_non_digit x1) => (SmtTerm.str_indexof_re (__eo_to_smt x1) (SmtTerm.re_comp (SmtTerm.re_range (SmtTerm.String (native_string_lit "0")) (SmtTerm.String (native_string_lit "9")))) (SmtTerm.Numeral 0))
-  | (Term.Apply (Term.UOp1 UserOp1._at_strings_itos_result x1) x2) => (SmtTerm.mod (__eo_to_smt x1) (SmtTerm.multmult (SmtTerm.Numeral 10) (__eo_to_smt x2)))
+  | (Term.Apply (Term.Apply (Term.UOp UserOp._at_strings_stoi_result) x1) x2) => (SmtTerm.str_to_int (SmtTerm.str_substr (__eo_to_smt x1) (SmtTerm.Numeral 0) (__eo_to_smt x2)))
+  | (Term.Apply (Term.UOp UserOp._at_strings_stoi_non_digit) x1) => (SmtTerm.str_indexof_re (__eo_to_smt x1) (SmtTerm.re_comp (SmtTerm.re_range (SmtTerm.String (native_string_lit "0")) (SmtTerm.String (native_string_lit "9")))) (SmtTerm.Numeral 0))
+  | (Term.Apply (Term.Apply (Term.UOp UserOp._at_strings_itos_result) x1) x2) => (SmtTerm.mod (__eo_to_smt x1) (SmtTerm.multmult (SmtTerm.Numeral 10) (__eo_to_smt x2)))
   | (Term.Apply (Term.Apply (Term.UOp UserOp._at_strings_num_occur) x1) x2) => 
     let _v0 := (__eo_to_smt x2)
     let _v1 := (__eo_to_smt x1)
@@ -405,7 +405,7 @@ def __eo_to_smt : Term -> SmtTerm
     (SmtTerm.eq _v0 (SmtTerm.set_singleton (SmtTerm.map_diff _v0 (SmtTerm.set_empty (__eo_to_smt_set_elem_type (__smtx_typeof _v0))))))
   | (Term.Apply (Term.Apply (Term.UOp UserOp.set_insert) Term.__eo_List_nil) x1) => SmtTerm.None
   | (Term.Apply (Term.Apply (Term.UOp UserOp.set_insert) x1) x2) => (__eo_to_smt_set_insert x1 (__eo_to_smt x2))
-  | (Term.UOp2 UserOp2._at_sets_deq_diff x1 x2) => 
+  | (Term.Apply (Term.Apply (Term.UOp UserOp._at_sets_deq_diff) x1) x2) => 
     let _v0 := (__eo_to_smt x2)
     let _v1 := (__eo_to_smt x1)
     (__eo_to_smt_sets_deq_diff _v1 (__smtx_typeof _v1) _v0 (__smtx_typeof _v0))
